verif/HMAC.v
@@ -26,4 +26,5 @@ Definition whole_prog :=
 Definition ge := bind_decl_groups whole_prog gempty.
 
 
-  
+Definition hmacSHA256 : ident := (352,"hmacSHA256").
+Definition hmac : ident := (354,"hmac").
