verif/HMACProof.v
@@ -4,7 +4,7 @@ Require Import String.
 
 (* Borrow from CompCert *)
 Require Import Coqlib.
-Require Import Integers.
+Require Import Bitvectors.
 
 Require Import AST.
 Require Import Semantics.
@@ -13,9 +13,37 @@ Require Import Builtins.
 Require Import BuiltinSem.
 Require Import Values.        
 
-Require Import Tactics.
+Require Import EvalTac.
 
 Require Import HMAC.
+Require Import HMACSpec.
 
 (* TODO: here will be a proof about HMAC *)
 (* relating the cryptol implementation to the spec *)
+
+Definition lzero := EList ((ETApp (ETApp (EVar (0,"demote")) (TCon (TC (TCNum 0)) nil)) (TCon (TC (TCNum 8)) nil)) :: nil).
+
+Definition t := TCon (TC (TCNum 1)) nil.
+
+Definition call_hmac_on_zero := EApp (EApp (ETApp (ETApp (EVar hmacSHA256) t) t) lzero) lzero.
+
+Lemma eval_hmac_sha256 :
+  exists v,
+    eval_expr ge empty call_hmac_on_zero v.
+Proof.
+  
+  eexists.
+  e. e. e. e.
+  g.
+  e. e. e. e.
+  e. e. e. e. e. e.
+  e. e. e. e. e.
+  e. e. e.
+  e. do 10 e.
+  e. e. e.
+  e. e. e. e. e.
+  e. e. e. e. e. e. g.
+  e. e. e. e. e. e. e. e. e. e.
+  repeat e. repeat e.
+  
+Admitted.
