src/BuiltinSem.v
@@ -37,49 +37,49 @@ Definition table : list (string * Expr) :=
   ("*", mb 1 2 Times) :: (* TESTED *)
   ("/", mb 1 2 Div) :: (* TESTED *)
   ("%", mb 1 2 Mod) :: (* TESTED *)
-  ("^^", mb 1 2 Exp) ::
-  ("lg2", mb 1 2 lg2) ::
+  ("^^", mb 1 2 Exp) :: (* Underlying op not implemented *)
+  ("lg2", mb 1 2 lg2) :: (* Underlying op not implemented *)
   ("True", mb 0 0 true_builtin) :: (* TESTED *)
   ("False", mb 0 0 false_builtin) :: (* TESTED *)
   ("negate", mb 1 1 Neg) :: (* TESTED *)
   ("complement", mb 1 1 Compl) :: (* TESTED *)
-  ("<", mb 1 2 Lt) ::
-  (">", mb 1 2 Gt) ::
-  ("<=", mb 1 2 Le) ::
-  (">=", mb 1 2 Ge) ::
-  ("==", mb 1 2 Eq) ::
-  ("!=", mb 1 2 Neq) ::
-  ("&&", mb 1 2 And) ::
-  ("||", mb 1 2 Or) ::
-  ("^", mb 1 2 Xor) ::
-  ("zero", mb 1 0 Zero) ::
-  ("<<", mb 1 2 Shiftl) ::
-  (">>", mb 1 2 Shiftr) ::
-  ("<<<", mb 1 2 Rotl) ::
-  (">>>", mb 1 2 Rotr) ::
-  ("#", mb 3 2 Append) ::
-  ("splitAt", mb 3 1 splitAt) ::
-  ("join", mb 9 9 join) ::
-  ("split", mb 3 1 split) ::
-  ("reverse", mb 9 9 reverse) ::
-  ("transpose", mb 9 9 transpose) ::
-  ("@", mb 3 2 At) ::
-  ("@@", mb 9 9 AtAt) ::
-  ("!", mb 9 9 Bang) ::
-  ("!!", mb 9 9 BangBang) ::
-  ("update", mb 9 9 update) ::
-  ("updateEnd", mb 9 9 updateEnd) ::
-  ("fromThen", mb 9 9 fromThen) ::
-  ("fromTo", mb 9 9 fromTo) ::
-  ("fromThenTo", mb 9 9 fromThenTo) ::
-  ("infFrom", mb 9 9 infFrom) ::
-  ("infFromThen", mb 9 9 infFromThen) ::
-  ("error", mb 9 9 error) ::
-  ("pmult", mb 9 9 pmult) ::
-  ("pdiv", mb 9 9 pdiv) ::
-  ("pmod", mb 9 9 pmod) ::
-  ("random", mb 9 9 random) ::
-  ("trace", mb 9 9 trace) ::
+  ("<", mb 1 2 Lt) :: (* Implemented, needs testing *)
+  (">", mb 1 2 Gt) :: (* Implemented, needs testing *)
+  ("<=", mb 1 2 Le) :: (* Implemented, needs testing *)
+  (">=", mb 1 2 Ge) :: (* Implemented, needs testing *)
+  ("==", mb 1 2 Eq) :: (* Implemented, needs testing *)
+  ("!=", mb 1 2 Neq) :: (* Implemented, needs testing *)
+  ("&&", mb 1 2 And) :: (* Implemented, needs testing *)
+  ("||", mb 1 2 Or) :: (* Implemented, needs testing *)
+  ("^", mb 1 2 Xor) :: (* Implemented, needs testing *)
+  ("zero", mb 1 0 Zero) :: (* Partially implemented, needs testing (and full implementation) *)
+  ("<<", mb 1 2 Shiftl) :: (* Implemented, needs testing *)
+  (">>", mb 1 2 Shiftr) :: (* Implemented, needs testing *)
+  ("<<<", mb 1 2 Rotl) :: (* Implemented, needs testing *)
+  (">>>", mb 1 2 Rotr) :: (* Implemented, needs testing *)
+  ("#", mb 3 2 Append) :: (* TESTED *)
+  ("splitAt", mb 3 1 splitAt) :: (* TESTED *)
+  ("join", mb 9 9 join) :: (* Not yet implemented *)
+  ("split", mb 3 1 split) :: (* TESTED *)
+  ("reverse", mb 9 9 reverse) :: (* Not yet implemented *)
+  ("transpose", mb 9 9 transpose) :: (* Not yet implemented *)
+  ("@", mb 3 2 At) :: (* TESTED *)
+  ("@@", mb 9 9 AtAt) :: (* Not yet implemented *)
+  ("!", mb 9 9 Bang) :: (* Not yet implemented *)
+  ("!!", mb 9 9 BangBang) :: (* Not yet implemented *)
+  ("update", mb 9 9 update) ::(* Not yet implemented *)
+  ("updateEnd", mb 9 9 updateEnd) :: (* Not yet implemented *)
+  ("fromThen", mb 9 9 fromThen) :: (* Not yet implemented *)
+  ("fromTo", mb 9 9 fromTo) :: (* Not yet implemented *)
+  ("fromThenTo", mb 9 9 fromThenTo) :: (* Not yet implemented *)
+  ("infFrom", mb 9 9 infFrom) :: (* Not yet implemented *)
+  ("infFromThen", mb 9 9 infFromThen) :: (* Not yet implemented *)
+  ("error", mb 9 9 error) :: (* Not yet implemented *)
+  ("pmult", mb 9 9 pmult) :: (* Not yet implemented *)
+  ("pdiv", mb 9 9 pdiv) :: (* Not yet implemented *)
+  ("pmod", mb 9 9 pmod) :: (* Not yet implemented *)
+  ("random", mb 9 9 random) :: (* Not yet implemented *)
+  ("trace", mb 9 9 trace) :: (* Not yet implemented *)
   nil.
 
 Fixpoint lookup {A : Type} (s : string) (t : list (string * A)) : option A :=
