src/Values.v
@@ -6,12 +6,14 @@ Inductive val :=
 | bit (b : bool) (* Can we ever get this now? *)
 | bits {n} (b : BitV n) (* bitvector *)
 | close (id : ident) (e : Expr) (E : ident -> option val)  (* closure *)
+| tclose (id : ident) (e : Expr) (E : ident -> option val) (* type closure *)
 | tuple (l : list val) (* heterogeneous tuples *)
 | rec (l : list (string * val)) (* records *)
 | typ (t : Typ) (* type value, used to fill in type variables *)
-| tclose (id : ident) (e : Expr) (E : ident -> option val) (* type closure *)
 | vcons (v : val) (e : Expr) (E : ident -> option val) (* lazy list: first val computed, rest is thunked *)
 | vnil (* empty list *)
+.
+(*
 | vcomp (e : Expr) (E : ident -> option val) (l : list (list Match)) (* lazy list comprehension *)
 | vapp (l1 l2 : Expr) (E : ident -> option val)
 | vsplit (n m : Z) (l : Expr) (E : ident -> option val)
@@ -23,6 +25,7 @@ Inductive val :=
 (* only then would you do any computation on the lazy list *)
 | vslice (l h : nat) (e : Expr) (E : ident -> option val)
 .
+ *)
 
 Definition env := ident -> option val.
 Definition empty : env := fun _ => None.
